POR_examples.v
@@ -1,0 +1,198 @@
+
+From Coq Require Import String Bool.
+
+From SymEx Require Import Expr.
+Import BasicExpr.
+
+From SymEx Require Import Parallel Traces.
+Import TraceSemantics.
+
+From SymEx Require Import Maps.
+Import BasicMaps.
+
+From SymEx Require Import ContextReduction PartialOrderReduction.
+
+Open Scope com_scope.
+Open Scope trace_scope.
+
+Example par_simple_0: red__S ([], <{ (X := 1 ; Y := 1 || Y := 2) || X := 2}>)
+                        ([Asgn__S X 1], <{ (skip ; Y := 1 || Y := 2) || X := 2 }>).
+Proof. apply ctx_red_intro with (C := fun x => <{ (x ; Y := 1 || Y := 2) || X := 2}>); repeat constructor. Qed.
+
+Example par_simple_1: red__S ([Asgn__S X 1], <{ (Y := 1 || Y := 2) || X := 2 }>)
+                        ([Asgn__S X 1 ; Asgn__S Y 2], <{ (Y := 1 || skip) || X := 2 }>).
+Proof. apply ctx_red_intro with (C := fun x => <{ (Y := 1 || x) || X := 2 }>); repeat constructor. Qed.
+
+Example par_simple_2: red__S ([Asgn__S X 1 ; Asgn__S Y 2], <{ Y := 1 || X := 2 }>)
+                        ([Asgn__S X 1 ; Asgn__S Y 2 ; Asgn__S X 2], <{ Y := 1 || skip }>).
+Proof. eapply ctx_red_intro; repeat constructor. Qed.
+
+Example par_simple_3: red__S ([Asgn__S X 1 ; Asgn__S Y 2 ; Asgn__S X 2], <{ Y := 1 }>)
+                        ([Asgn__S X 1 ; Asgn__S Y 2 ; Asgn__S X 2 ; Asgn__S Y 1], <{ skip }>) .
+Proof. eapply ctx_red_intro with (C := fun x => x); repeat constructor. Qed.
+
+Example par_simple: red_star__S ([], <{ (X := 1 ; Y := 1 || Y := 2) || X := 2}>)
+                      ([Asgn__S X 1 ; Asgn__S Y 2 ; Asgn__S X 2 ; Asgn__S Y 1], <{ skip }>).
+Proof.
+  econstructor. apply par_simple_3.
+  econstructor. apply ctx_red_intro with (C := fun x => x). apply head_red_skip_par_r__S. constructor.
+  econstructor. apply par_simple_2.
+  econstructor. apply ctx_red_intro with (C := fun x => <{ x || X := 2 }>);
+    [ apply head_red_skip_par_r__S| repeat constructor].
+  econstructor. apply par_simple_1.
+  econstructor. apply ctx_red_intro with (C := fun x => <{ x || X := 2 }>);
+    [ apply head_red_skip_seq__S | repeat constructor].
+  econstructor. apply par_simple_0.
+  constructor.
+Qed.
+
+Definition final_trace (s: Stmt) (t: trace__S): Prop := red_star__S ([], s) (t, SSkip).
+
+Example example2_stmt: Stmt := <{ Y := X || Z := X || X := 2 }>.
+
+Example example2_t1: final_trace example2_stmt [Asgn__S Y X ; Asgn__S Z X ; Asgn__S X 2].
+Proof.
+  apply Relation_Operators.rtn1_trans with
+    (y := ([Asgn__S Y X;Asgn__S Z X], <{ X := 2 }>)).
+  apply ctx_red_intro with (C := fun s => s); constructor.
+  apply Relation_Operators.rtn1_trans with
+    (y := ([Asgn__S Y X;Asgn__S Z X], <{skip || X := 2}>)).
+  apply ctx_red_intro with (C := fun s => s); constructor.
+  apply Relation_Operators.rtn1_trans with
+    (y := ([Asgn__S Y X], <{ Z := X || X := 2}>)).
+  apply ctx_red_intro with (C := fun s => <{ s || X := 2 }>); repeat constructor.
+  apply Relation_Operators.rtn1_trans with
+    (y := ([Asgn__S Y X], <{ skip || Z := X || X := 2}>)).
+  apply ctx_red_intro with (C := fun s => s); repeat constructor.
+  apply Relation_Operators.rtn1_trans with
+    (y := ([], <{ Y := X || Z := X || X := 2}>)).
+  apply ctx_red_intro with (C := fun s => <{ s || Z := X || X := 2 }>); repeat constructor.
+  constructor.
+Qed.
+
+Example example2_t2: final_trace example2_stmt [Asgn__S Z X ; Asgn__S Y X ; Asgn__S X 2].
+Proof.
+  apply Relation_Operators.rtn1_trans with
+    (y := ([Asgn__S Z X;Asgn__S Y X], <{ X := 2 }>)).
+  apply ctx_red_intro with (C := fun s => s); constructor.
+  apply Relation_Operators.rtn1_trans with
+    (y := ([Asgn__S Z X;Asgn__S Y X], <{skip || X := 2}>)).
+  apply ctx_red_intro with (C := fun s => s); constructor.
+  apply Relation_Operators.rtn1_trans with
+    (y := ([Asgn__S Z X;Asgn__S Y X], <{skip || skip || X := 2}>)).
+  apply ctx_red_intro with (C := fun s => s); repeat constructor.
+  apply Relation_Operators.rtn1_trans with
+    (y := ([Asgn__S Z X], <{ Y := X || skip || X := 2}>)).
+  apply ctx_red_intro with (C := fun s => <{s || skip || X := 2}>); repeat constructor.
+  apply Relation_Operators.rtn1_trans with
+    (y := ([], <{ Y := X || Z := X || X := 2}>)).
+  apply ctx_red_intro with (C := fun s => <{Y := X || s || X := 2}>); repeat constructor.
+  constructor.
+Qed.
+
+Example example2_t3: final_trace example2_stmt [Asgn__S Y X ; Asgn__S X 2 ; Asgn__S Z X].
+Proof.
+  apply Relation_Operators.rtn1_trans with
+    (y := ([Asgn__S Y X ; Asgn__S X 2 ; Asgn__S Z X], <{ skip || skip }>)).
+  apply ctx_red_intro with (C := fun s => s); constructor.
+  apply Relation_Operators.rtn1_trans with
+    (y := ([Asgn__S Y X ; Asgn__S X 2 ; Asgn__S Z X], <{ skip || skip || skip }>)).
+  apply ctx_red_intro with (C := fun s => s); constructor.
+  apply Relation_Operators.rtn1_trans with
+    (y := ([Asgn__S Y X ; Asgn__S X 2], <{ skip || Z := X || skip }>)).
+  apply ctx_red_intro with (C := fun s => <{ skip || s || skip }>); repeat constructor.
+  apply Relation_Operators.rtn1_trans with
+    (y := ([Asgn__S Y X], <{ skip || Z := X || X := 2 }>)).
+  apply ctx_red_intro with (C := fun s => <{ skip || Z := X || s }>); repeat constructor.
+  apply Relation_Operators.rtn1_trans with
+    (y := ([], <{ Y := X || Z := X || X := 2 }>)).
+  apply ctx_red_intro with (C := fun s => <{ s || Z := X || X := 2 }>); repeat constructor.
+  constructor.
+Qed.
+
+Example example2_t4: final_trace example2_stmt [Asgn__S Z X ; Asgn__S X 2 ; Asgn__S Y X].
+Proof.
+  apply Relation_Operators.rtn1_trans with
+    (y := ([Asgn__S Z X ; Asgn__S X 2 ; Asgn__S Y X], <{ skip || skip }>)).
+  apply ctx_red_intro with (C := fun s => s); constructor.
+  apply Relation_Operators.rtn1_trans with
+    (y := ([Asgn__S Z X ; Asgn__S X 2 ; Asgn__S Y X], <{ skip || skip || skip }>)).
+  apply ctx_red_intro with (C := fun s => s); constructor.
+  apply Relation_Operators.rtn1_trans with
+    (y := ([Asgn__S Z X ; Asgn__S X 2], <{ Y := X || skip || skip }>)).
+  apply ctx_red_intro with (C := fun s => <{s || skip || skip}>); repeat constructor.
+  apply Relation_Operators.rtn1_trans with
+    (y := ([Asgn__S Z X], <{ Y := X || skip || X := 2 }>)).
+  apply ctx_red_intro with (C := fun s => <{Y := X || skip || s}>); repeat constructor.
+  apply Relation_Operators.rtn1_trans with
+    (y := ([], <{ Y := X || Z := X || X := 2 }>)).
+  apply ctx_red_intro with (C := fun s => <{Y := X || s || X := 2}>); repeat constructor.
+  constructor.
+Qed.
+
+Example example2_t5: final_trace example2_stmt [Asgn__S X 2 ; Asgn__S Y X ; Asgn__S Z X].
+Proof.
+  apply Relation_Operators.rtn1_trans with
+    (y := ([Asgn__S X 2 ; Asgn__S Y X ; Asgn__S Z X], <{ skip || skip }>)).
+  apply ctx_red_intro with (C := fun s => s); constructor.
+  apply Relation_Operators.rtn1_trans with
+    (y := ([Asgn__S X 2 ; Asgn__S Y X ; Asgn__S Z X], <{ skip || skip || skip }>)).
+  apply ctx_red_intro with (C := fun s => s); constructor.
+  apply Relation_Operators.rtn1_trans with
+    (y := ([Asgn__S X 2 ; Asgn__S Y X], <{ skip || Z := X || skip }>)).
+  apply ctx_red_intro with (C := fun s => <{skip || s || skip}>); repeat constructor.
+  apply Relation_Operators.rtn1_trans with
+    (y := ([Asgn__S X 2], <{ Y := X || Z := X || skip }>)).
+  apply ctx_red_intro with (C := fun s => <{s || Z := X || skip}>); repeat constructor.
+  apply Relation_Operators.rtn1_trans with
+    (y := ([], <{ Y := X || Z := X || X := 2 }>)).
+  apply ctx_red_intro with (C := fun s => <{ Y := X || Z := X || s}>); repeat constructor.
+  constructor.
+Qed.
+
+Example example2_t6: final_trace example2_stmt [Asgn__S X 2 ; Asgn__S Z X ; Asgn__S Y X].
+Proof.
+  apply Relation_Operators.rtn1_trans with
+    (y := ([Asgn__S X 2 ; Asgn__S Z X ; Asgn__S Y X], <{ skip || skip }>)).
+  apply ctx_red_intro with (C := fun s => s); constructor.
+  apply Relation_Operators.rtn1_trans with
+    (y := ([Asgn__S X 2 ; Asgn__S Z X ; Asgn__S Y X], <{ skip || skip || skip }>)).
+  apply ctx_red_intro with (C := fun s => s); constructor.
+  apply Relation_Operators.rtn1_trans with
+    (y := ([Asgn__S X 2 ; Asgn__S Z X], <{ Y := X || skip || skip }>)).
+  apply ctx_red_intro with (C := fun s => <{s || skip || skip}>); repeat constructor.
+  apply Relation_Operators.rtn1_trans with
+    (y := ([Asgn__S X 2], <{ Y := X || Z := X || skip }>)).
+  apply ctx_red_intro with (C := fun s => <{ Y := X || s || skip}>); repeat constructor.
+  apply Relation_Operators.rtn1_trans with
+    (y := ([], <{ Y := X || Z := X || X := 2 }>)).
+  apply ctx_red_intro with (C := fun s => <{ Y := X || Z := X || s}>); repeat constructor.
+  constructor.
+Qed.
+
+Example example_IF: interference_free (Asgn__S Z X) (Asgn__S Y X).
+Proof. splits; unfold reads_var, writes_var, contains__A; intro contra;
+         destruct contra; subst; discriminate.
+Qed.
+
+Definition final_trace__POR (s: Stmt) (t: trace__S): Prop := red_star__POR ([], s) (t, SSkip).
+
+Example example2_t1__POR: final_trace__POR example2_stmt [Asgn__S Y X ; Asgn__S Z X ; Asgn__S X 2].
+Proof.
+  apply Relation_Operators.rtn1_trans with
+    (y := ([Asgn__S Y X ; Asgn__S Z X ; Asgn__S X 2], <{ skip || skip }>)).
+  apply ctx_red_intro with (C := fun s => s); repeat econstructor.
+  apply Relation_Operators.rtn1_trans with
+    (y := ([Asgn__S Y X ; Asgn__S Z X ; Asgn__S X 2], <{ skip || skip || skip }>)).
+  apply ctx_red_intro with (C := fun s => s); repeat econstructor.
+  apply Relation_Operators.rtn1_trans with
+    (y := ([Asgn__S Y X ; Asgn__S Z X], <{ skip || skip || X := 2 }>)).
+  apply ctx_red_intro with (C := fun s => <{skip || skip || s}>); repeat econstructor.
+  apply Relation_Operators.rtn1_trans with
+    (y := ([Asgn__S Y X], <{ skip || Z := X || X := 2 }>)).
+  apply ctx_red_intro with (C := fun s => <{skip || s || X := 2}>); repeat econstructor.
+  apply Relation_Operators.rtn1_trans with
+    (y := ([], <{ Y := X || Z := X || X := 2 }>)).
+  apply ctx_red_intro with (C := fun s => <{s || _ || _}>); repeat econstructor.
+  constructor.
+Qed.
