README.md
@@ -23,15 +23,16 @@ coq_makefile -f _CoqProject -o Makefile
 The approach to syntax and transition relation semantics is based on [Programming Language Foundations](https://softwarefoundations.cis.upenn.edu/plf-current/index.html)
 
 ### Extensions
-- [TraceSemantics](./TraceSemantics.v) introduces trace semantics for the language with procedures
+- [Trace Semantics](./TraceSemantics.v) introduces trace semantics for the language with procedures
   - Notation and lemmas about traces are in [Traces](./Traces.v)
   - Some examples of programs and their traces are found in [examples](./Trace_examples.v)
-- [ParallelTraces](./ParallelTraces.v) adds a parallel composition operator to the base language with trace semantics.
+- [Parallel Traces](./ParallelTraces.v) adds a parallel composition operator to the base language with trace semantics.
 Additionally contains some preliminary results about reduction of trace sets.
     - The base language with a parallel operator is in [Parallel](./Parallel.v)
-- [ContextReduction](./ContextReduction) contains an alternative approach to syntax based on reductions in a context inspired by [Mechanized Semantics](https://github.com/xavierleroy/cdf-mech-sem)
-- [SymPaths](./SymPaths.v) formalizes [partial order reduction](https://rdcu.be/c58yn) of symbolic execution in the context reduction style
-- [SimpleParallelLogic](./SimpleParallelLogic.v) contains some notes on a context-reduction logic for [Parallel](./Parallel.v)
+- [Context Reduction](./ContextReduction) contains an alternative approach to syntax based on reductions in a context inspired by [Mechanized Semantics](https://github.com/xavierleroy/cdf-mech-sem)
+- [Partial Order Reduction](./PartialOrderReduction.v) formalizes [partial order reduction](https://rdcu.be/c58yn) of symbolic execution in the context reduction style
+  - Some examples of programs and their traces with and without POR are found in [examples](./POR_examples.v)
+- [Program Logics](./ProgramLogics.v) contains some notes on program logics for [Parallel](./Parallel.v). In particular the DL from sympaths and Einar's simple parallel logic
 
 ### Other
 - [PLACES](./PLACES) contains a talk proposal to [PLACES 2023](https://places-workshop.github.io/2023/)
